added state to eval_aexp. Also refactored id into a separate ident module and added an eval module that contains the evaluation methods and depends on sigma, aexp, bexp, etc. Also added variables to aexp.

Bexp.v
@@ -11,31 +11,7 @@ Inductive Bexp :=
   | And: Bexp -> Bexp -> Bexp
   | Or: Bexp -> Bexp -> Bexp.
 
-Fixpoint eval_bexp (b: Bexp): BexpLit :=
-  match b with
-    | Lit b' => b'
-    | Not a => match eval_bexp a with
-        | true => false
-        | false => true
-      end
-    | And a b => match (eval_bexp a, eval_bexp b) with
-        | (true, true) => true
-        | _ => false
-      end
-    | Or a b => match (eval_bexp a, eval_bexp b) with
-        | (false, false) => false
-        | _ => true
-      end
-  end.
-
 End Bexp.
 
 Export Bexp.
 
-(** Some tests *)
-Example t1_expr := Or (Lit false) (And (Not (Lit false)) (Lit true)).
-Example f1_expr := Or (Lit false) (And (Lit false) (Lit true)).
-Example t1_eval: eval_bexp t1_expr = true.
-Proof. compute; reflexivity. Qed.
-Example f1_eval: eval_bexp f1_expr = false.
-Proof. compute; reflexivity. Qed.
