Eval.v
@@ -1,0 +1,49 @@
+(* Contains the code that actually evaluates expressions and commands *)
+
+Require Export Typ.
+Require Export Sigma.
+Require Export Aexp.
+Require Export Bexp.
+
+Module Eval.
+
+Fixpoint eval_aexp (a : Aexp) (sigma : state) :=
+  match a with
+    | ALit a' => a'
+    | APlus b c => plus_aexplit (eval_aexp b sigma) (eval_aexp c sigma)
+    | AMinus b c => minus_aexplit (eval_aexp b sigma) (eval_aexp c sigma)
+    | AMult b c => mult_aexplit (eval_aexp b sigma) (eval_aexp c sigma)
+    | ADiv b c => div_aexplit (eval_aexp b sigma) (eval_aexp c sigma)
+    | AExp b c => exp_aexplit (eval_aexp b sigma) (eval_aexp c sigma)
+    | ANeg b => neg_aexplit (eval_aexp b sigma)
+    | AVar i => match (sigma i) with | mk_typ _ t => match t with | aexplit a' => a' (*| _ => aexplit_zero (*error!*)*) end end
+  end.
+
+Fixpoint eval_bexp (b: Bexp): BexpLit :=
+  match b with
+    | Lit b' => b'
+    | Not a => match eval_bexp a with
+        | true => false
+        | false => true
+      end
+    | And a b => match (eval_bexp a, eval_bexp b) with
+        | (true, true) => true
+        | _ => false
+      end
+    | Or a b => match (eval_bexp a, eval_bexp b) with
+        | (false, false) => false
+        | _ => true
+      end
+  end.
+
+(** Some tests for bexp eval *)
+Example t1_expr := Or (Lit false) (And (Not (Lit false)) (Lit true)).
+Example f1_expr := Or (Lit false) (And (Lit false) (Lit true)).
+Example t1_eval: eval_bexp t1_expr = true.
+Proof. compute; reflexivity. Qed.
+Example f1_eval: eval_bexp f1_expr = false.
+Proof. compute; reflexivity. Qed.
+
+End Eval.
+
+Export Eval.
