Ident.v
@@ -1,0 +1,20 @@
+(* Kodellama identifiers are strings! *)
+
+Require Export String.
+
+Module Ident.
+
+Inductive ident :=
+  | mk_id : string -> ident.
+
+Definition beq_str (s1 s2 : string) : bool :=
+  andb (prefix s1 s2) (EqNat.beq_nat (length s1) (length s2)).
+
+Definition beq_ident (i1 i2 : ident) : bool :=
+  match i1, i2 with
+    | mk_id s1, mk_id s2 => beq_str s1 s2
+  end.
+
+End Ident.
+
+Export Ident.
