Sigma.v
@@ -1,25 +1,14 @@
 (* This module contains the basic state of a KodeLlama2 program that's running *)
 
 Require Export Typ.
-Require Export String.
+Require Export Ident.
 
 Module Sigma.
 
-Inductive id :=
-  | mk_id : string -> id.
+Definition state := ident -> typ.
 
-Definition beq_str (s1 s2 : string) : bool :=
-  andb (prefix s1 s2) (EqNat.beq_nat (length s1) (length s2)).
-
-Definition beq_id (i1 i2 : id) : bool :=
-  match i1, i2 with
-    | mk_id s1, mk_id s2 => beq_str s1 s2
-  end.
-
-Definition state := id -> typ.
-
-Definition update (sigma : state) (i : id) (t : typ) : state :=
-  fun i' => if beq_id i i' 
+Definition update (sigma : state) (i : ident) (t : typ) : state :=
+  fun i' => if beq_ident i i' 
     then match (sigma i) with
       | mk_typ b _ => if b then (sigma i) else t end  
     else sigma i'.
